

Lemma L1: Fourier Coefficient Formula

Alethfeld Verified Proof

Alethfeld Proof Orchestrator v4

Verification Status: **VERIFIED** | Taint: **CLEAN**

Dependencies

Assumption 1 (A1: Product State QBF). Let $U = I - 2|\psi\rangle\langle\psi|$ be a rank-1 quantum Boolean function where $|\psi\rangle = \bigotimes_{k=1}^n |\phi_k\rangle$ is a product state.

Definition 1 (D1: Bloch Vector). For each qubit k , the Bloch vector $\vec{r}_k = (x_k, y_k, z_k)$ satisfies $|\vec{r}_k|^2 = 1$. Define extended Bloch components:

$$r_k^{(0)} = 1, \quad r_k^{(1)} = x_k, \quad r_k^{(2)} = y_k, \quad r_k^{(3)} = z_k.$$

Statement

Lemma 1 (Fourier Coefficient Formula). *Under Assumption 1 and Definition 1, for any multi-index $\alpha \in \{0, 1, 2, 3\}^n$:*

$$\hat{U}(\alpha) = \delta_{\alpha,0} - 2^{1-n} \prod_{k=1}^n r_k^{(\alpha_k)}$$

where $\delta_{\alpha,0} = 1$ if $\alpha = (0, \dots, 0)$ and 0 otherwise.

Proof

Step 1: Definition Expansion

Claim 1 (L1-step1). $\hat{U}(\alpha) = 2^{-n} \text{Tr}(\sigma^\alpha U) = 2^{-n} \text{Tr}(\sigma^\alpha) - 2^{1-n} \text{Tr}(\sigma^\alpha |\psi\rangle\langle\psi|)$

Proof. By definition of the Pauli-Fourier coefficient, $\hat{U}(\alpha) = 2^{-n} \text{Tr}(\sigma^\alpha U)$. Substituting $U = I - 2|\psi\rangle\langle\psi|$ from Assumption 1:

$$\hat{U}(\alpha) = 2^{-n} \text{Tr}(\sigma^\alpha (I - 2|\psi\rangle\langle\psi|)) = 2^{-n} \text{Tr}(\sigma^\alpha) - 2^{1-n} \text{Tr}(\sigma^\alpha |\psi\rangle\langle\psi|). \quad \square$$

Step 2: Trace of Pauli String

Claim 2 (L1-step2). $\text{Tr}(\sigma^\alpha) = 2^n \delta_{\alpha,0}$

Proof. We proceed in substeps.

(2a) By definition, $\sigma^\alpha = \sigma^{\alpha_1} \otimes \sigma^{\alpha_2} \otimes \dots \otimes \sigma^{\alpha_n}$.

(2b) For tensor products, $\text{Tr}(A \otimes B) = \text{Tr}(A) \cdot \text{Tr}(B)$.

(2b.1) By definition, $(A \otimes B)_{(i,j),(k,l)} = A_{ik}B_{jl}$.

(2b.2) Thus $\text{Tr}(A \otimes B) = \sum_{i,j} (A \otimes B)_{(i,j),(i,j)} = \sum_{i,j} A_{ii}B_{jj} = \text{Tr}(A) \text{Tr}(B)$.

(2c) Applying (2a) and (2b) inductively: $\text{Tr}(\sigma^\alpha) = \prod_{k=1}^n \text{Tr}(\sigma^{\alpha_k})$.

(2d) For single-qubit Pauli matrices:

(2d.1) $\sigma^0 = I_2 = \begin{pmatrix} 1 & 0 \\ 0 & 1 \end{pmatrix}$, so $\text{Tr}(\sigma^0) = 2$.

(2d.2) $\sigma^1 = \sigma_x = \begin{pmatrix} 0 & 1 \\ 1 & 0 \end{pmatrix}$, so $\text{Tr}(\sigma^1) = 0$.

(2d.3) $\sigma^2 = \sigma_y = \begin{pmatrix} 0 & -i \\ i & 0 \end{pmatrix}$, so $\text{Tr}(\sigma^2) = 0$.

(2d.4) $\sigma^3 = \sigma_z = \begin{pmatrix} 1 & 0 \\ 0 & -1 \end{pmatrix}$, so $\text{Tr}(\sigma^3) = 0$.

(2e) Case analysis on the product:

(2e.1) If $\exists k : \alpha_k \neq 0$, then $\text{Tr}(\sigma^{\alpha_k}) = 0$, so the product vanishes.

(2e.2) If $\forall k : \alpha_k = 0$, then each factor equals 2, giving 2^n .

Therefore $\text{Tr}(\sigma^\alpha) = 2^n \delta_{\alpha,0}$. □

Step 3: Trace Cyclic Property

Claim 3 (L1-step3). $\text{Tr}(\sigma^\alpha |\psi\rangle \langle \psi|) = \langle \psi | \sigma^\alpha | \psi \rangle$

Proof. **(3a)** The operator $|\psi\rangle \langle \psi|$ is a rank-1 projector.

(3c) For any operator A and normalized state $|\psi\rangle$:

(3c.1) Let $\{|e_j\rangle\}$ be an orthonormal basis. Then

$$\text{Tr}(A |\psi\rangle \langle \psi|) = \sum_j \langle e_j | A | \psi \rangle \langle \psi | e_j \rangle.$$

(3c.2) Rearranging scalars: $= \sum_j \langle \psi | e_j \rangle \langle e_j | A | \psi \rangle$.

(3c.3) By completeness ($\sum_j |e_j\rangle \langle e_j| = I$):

$$= \langle \psi | \left(\sum_j |e_j\rangle \langle e_j| \right) A | \psi \rangle = \langle \psi | A | \psi \rangle.$$

Setting $A = \sigma^\alpha$ yields the result. □

Step 4: Product State Factorization

Claim 4 (L1-step4). $\langle \psi | \sigma^\alpha | \psi \rangle = \prod_{k=1}^n \langle \phi_k | \sigma^{\alpha_k} | \phi_k \rangle = \prod_{k=1}^n r_k^{(\alpha_k)}$

Proof. (4a) From Assumption 1: $|\psi\rangle = |\phi_1\rangle \otimes \dots \otimes |\phi_n\rangle$ and $\sigma^\alpha = \sigma^{\alpha_1} \otimes \dots \otimes \sigma^{\alpha_n}$.

(4c) Tensor product operator action: $(A \otimes B)(|a\rangle \otimes |b\rangle) = (A|a\rangle) \otimes (B|b\rangle)$.

(4d) Tensor product inner product: $(\langle a| \otimes \langle b|)(|c\rangle \otimes |d\rangle) = \langle a|c\rangle \langle b|d\rangle$.

(4e) Combining (4c) and (4d) inductively:

$$\langle \psi | \sigma^\alpha | \psi \rangle = \prod_{k=1}^n \langle \phi_k | \sigma^{\alpha_k} | \phi_k \rangle.$$

(4f) For a single qubit $|\phi\rangle$ with Bloch vector (x, y, z) , parametrized as $|\phi\rangle = \cos(\theta/2)|0\rangle + e^{i\varphi} \sin(\theta/2)|1\rangle$ where $x = \sin \theta \cos \varphi$, $y = \sin \theta \sin \varphi$, $z = \cos \theta$:

$$(4f.2) \quad \langle \phi | I | \phi \rangle = 1 = r^{(0)}. \quad \checkmark$$

$$(4f.3) \quad \langle \phi | \sigma_x | \phi \rangle: \text{ Since } \sigma_x |\phi\rangle = \cos(\theta/2)|1\rangle + e^{i\varphi} \sin(\theta/2)|0\rangle,$$

$$\begin{aligned} \langle \phi | \sigma_x | \phi \rangle &= e^{-i\varphi} \sin(\theta/2) \cos(\theta/2) + e^{i\varphi} \cos(\theta/2) \sin(\theta/2) \\ &= 2 \cos(\theta/2) \sin(\theta/2) \cos \varphi = \sin \theta \cos \varphi = x = r^{(1)}. \quad \checkmark \end{aligned}$$

$$(4f.4) \quad \langle \phi | \sigma_y | \phi \rangle = \sin \theta \sin \varphi = y = r^{(2)}. \quad (\text{Analogous calculation.})$$

$$(4f.5) \quad \langle \phi | \sigma_z | \phi \rangle: \text{ Since } \sigma_z |0\rangle = |0\rangle \text{ and } \sigma_z |1\rangle = -|1\rangle,$$

$$\langle \phi | \sigma_z | \phi \rangle = \cos^2(\theta/2) - \sin^2(\theta/2) = \cos \theta = z = r^{(3)}. \quad \checkmark$$

Therefore $\langle \phi_k | \sigma^{\alpha_k} | \phi_k \rangle = r_k^{(\alpha_k)}$ for each k . □

Conclusion

Proof of Lemma 1. Combining Steps 1–4:

$$\begin{aligned} \hat{U}(\alpha) &= 2^{-n} \text{Tr}(\sigma^\alpha) - 2^{1-n} \text{Tr}(\sigma^\alpha |\psi\rangle \langle \psi|) && (\text{Step 1}) \\ &= 2^{-n} \cdot 2^n \delta_{\alpha,0} - 2^{1-n} \langle \psi | \sigma^\alpha | \psi \rangle && (\text{Steps 2, 3}) \\ &= \delta_{\alpha,0} - 2^{1-n} \prod_{k=1}^n r_k^{(\alpha_k)} && (\text{Step 4}) \end{aligned}$$

as claimed. □

Alethfeld Verification Report

Graph ID: L1-fourier-verify-2024
Total Nodes: 46 (6 original + 40 expanded)
Max Depth: 5
Admitted Steps: 0
Taint Status: **CLEAN**